subtype signature to include tid

src/assign_mcl.lean
@@ -5,21 +5,26 @@ open mcl.mclk
 
 namespace assign_mcl
 
-def sig : signature
+def sigc : signature_core
 | "tid" := { scope := scope.tlocal, type := ⟨1, type.int⟩ }
 | _ := { scope := scope.global, type := ⟨1, type.int⟩ }
 
+def sig : signature := ⟨sigc, begin
+    split,
+    refl,
+    refl,
+end⟩
 
-lemma a_is_global : is_global (sig "a") := by apply eq.refl
-lemma tid_is_tlocal : is_tlocal (sig "tid") := by apply eq.refl
+lemma a_is_global : is_global (sig.val "a") := by apply eq.refl
+lemma tid_is_tlocal : is_tlocal (sig.val "tid") := by apply eq.refl
 
 -- TODO generate those proofs directly from signature
 -- make type classes out of those
 -- make name explicit in state.update
-def read_tid := (expression.tlocal_var "tid" (λ_, 0) (show type_of (sig "tid") = type.int, by apply eq.refl) (show (sig "tid").type.dim = 1, by apply eq.refl) tid_is_tlocal)
+def read_tid := (expression.tlocal_var "tid" (λ_, 0) (show type_of (sig.val "tid") = type.int, by apply eq.refl) (show (sig.val "tid").type.dim = 1, by apply eq.refl) tid_is_tlocal)
 
-instance : has_one (expression sig (type_of (sig "b"))) := begin
-    have : type_of (sig "b") = type.int := by apply eq.refl,
+instance : has_one (expression sig (type_of (sig.val "b"))) := begin
+    have : type_of (sig.val "b") = type.int := by apply eq.refl,
     rw this,
     apply_instance,
 end
@@ -88,7 +93,7 @@ ac.nth i → (s.map_active_threads ac f).threads.nth i = f (s.threads.nth i) := 
 end
 
 lemma store_access_elim_name {sig : signature} {n n_idx} {s : state n (memory $ parlang_mcl_tlocal sig) (parlang_mcl_global sig)} {var} {idx : vector (expression sig type.int) n_idx} 
-{t h₄} {h₃ : type_of (sig var) = t } {f} {t : fin n} {i} {ac₁ : vector bool n} {updates}
+{t h₄} {h₃ : type_of (sig.val var) = t } {f} {t : fin n} {i} {ac₁ : vector bool n} {updates}
 (h₁ : i ∉ accesses (vector.nth ((map_active_threads ac₁ (f ∘ map_list updates) s).threads) t)) 
 (h₂ : i.1 ≠ var) :
 i ∉ accesses (vector.nth ((map_active_threads ac₁ (f ∘ (mcl_store var idx h₃ h₄) ∘ map_list updates) s).threads) t) := begin
@@ -97,7 +102,7 @@ end
 
 
 lemma store_access_elim_idx {sig : signature} {n n_idx} {s : state n (memory $ parlang_mcl_tlocal sig) (parlang_mcl_global sig)} {var} {idx : vector (expression sig type.int) n_idx} 
-{t} {h₄ : ((sig var).type).dim = n_idx} {h₃ : type_of (sig var) = t } {f} {t : fin n} {i : mcl_address sig} {ac₁ : vector bool n} {updates}
+{t} {h₄ : ((sig.val var).type).dim = n_idx} {h₃ : type_of (sig.val var) = t } {f} {t : fin n} {i : mcl_address sig} {ac₁ : vector bool n} {updates}
 (h₂ : i.2.to_list ≠ (idx.map ((eval (((map_active_threads ac₁ (map_list updates) s).threads).nth t).tlocal))).to_list) 
 (h₁ : i ∉ accesses (vector.nth ((map_active_threads ac₁ (f ∘ map_list updates) s).threads) t)) :
 i ∉ accesses (vector.nth ((map_active_threads ac₁ (f ∘ (mcl_store var idx h₃ h₄) ∘ map_list updates) s).threads) t) := begin
@@ -105,7 +110,7 @@ i ∉ accesses (vector.nth ((map_active_threads ac₁ (f ∘ (mcl_store var idx 
 end
 
 lemma store_access_elim_idx' {sig : signature} {n n_idx} {s : state n (memory $ parlang_mcl_tlocal sig) (parlang_mcl_global sig)} {var} {idx : vector (expression sig type.int) n_idx} 
-{t} {h₄ : ((sig var).type).dim = n_idx} {h₃ : type_of (sig var) = t } {t : fin n} {i : mcl_address sig} {ac₁ : vector bool n} {updates}
+{t} {h₄ : ((sig.val var).type).dim = n_idx} {h₃ : type_of (sig.val var) = t } {t : fin n} {i : mcl_address sig} {ac₁ : vector bool n} {updates}
 (h₂ : i.2.to_list ≠ (idx.map ((eval (((map_active_threads ac₁ (map_list updates) s).threads).nth t).tlocal ))).to_list) 
 (h₁ : i ∉ accesses (vector.nth (s.threads) t)) :
 i ∉ accesses (vector.nth ((map_active_threads ac₁ ((mcl_store var idx h₃ h₄) ∘ map_list updates) s).threads) t) := begin
@@ -113,7 +118,7 @@ i ∉ accesses (vector.nth ((map_active_threads ac₁ ((mcl_store var idx h₃ h
 end
 
 lemma store_store_success {sig : signature} {i : mcl_address sig} {updates} {ts : thread_state (memory $ parlang_mcl_tlocal sig) (parlang_mcl_global sig)} 
-{dim} {idx : vector (expression sig type.int) dim} {var t} {h₁ : type_of (sig var) = t} {h₂ : ((sig var).type).dim = dim} 
+{dim} {idx : vector (expression sig type.int) dim} {var t} {h₁ : type_of (sig.val var) = t} {h₂ : ((sig.val var).type).dim = dim} 
 {f : thread_state (memory $ parlang_mcl_tlocal sig) (parlang_mcl_global sig) → thread_state (memory $ parlang_mcl_tlocal sig) (parlang_mcl_global sig)} : 
 i = ⟨var, vector_mpr h₂ (idx.map (eval (map_list updates ts).tlocal))⟩ → i ∈ ((f ∘ mcl_store var idx h₁ h₂ ∘ map_list updates) ts).stores := by sorry
 
@@ -139,7 +144,7 @@ set_option trace.check true
 -- question: should we limit ourselfs to global scope here?
 structure array_access (sig : signature) (var : string) (i : mcl_address sig) : Prop :=
 (var_eq : i.1 = var)
-(idx_len : i.2.length = (sig var).type.dim)
+(idx_len : i.2.length = (sig.val var).type.dim)
 -- (bound : list.forall₂ nat.lt i.2 (sig var).type.sizes.to_list)
 
 structure array_access_tid_to_idx (sig : signature) (var : string) (i : mcl_address sig) (n : ℕ) extends array_access sig var i : Prop :=
@@ -189,7 +194,7 @@ end
 
 instance {sig var i} : decidable (array_access sig var i) :=
   if var_eq : i.1 = var then
-    if idx_len : i.2.length = (sig var).type.dim then is_true ⟨var_eq, idx_len⟩
+    if idx_len : i.2.length = (sig.val var).type.dim then is_true ⟨var_eq, idx_len⟩
     --   if bound : list.forall₂ eq i.2 (sig var).type.sizes.to_list then is_true ⟨var_eq, idx_len, bound⟩
     --   else is_false (assume h : array_access sig var i, bound (array_access.bound h))
     else is_false (assume h : array_access sig var i, idx_len (array_access.idx_len h))
@@ -198,7 +203,7 @@ instance {sig var i} : decidable (array_access sig var i) :=
 instance ll {sig var i n} : decidable (array_access_tid_to_idx sig var i n) := sorry
 
 lemma store_global_success {sig : signature} {i : mcl_address sig} {updates} 
-{dim} {idx : vector (expression sig type.int) dim} {var₁ var₂ t} {h₁ : type_of (sig var₂) = t} {h₂}
+{dim} {idx : vector (expression sig type.int) dim} {var₁ var₂ t} {h₁ : type_of (sig.val var₂) = t} {h₂}
 {ts : thread_state (memory $ parlang_mcl_tlocal sig) (parlang_mcl_global sig)}
 {f : thread_state (memory $ parlang_mcl_tlocal sig) (parlang_mcl_global sig) → thread_state (memory $ parlang_mcl_tlocal sig) (parlang_mcl_global sig)} (a : array_access sig var₁ i) (h : var₁ = var₂) : ((
         f ∘
@@ -207,11 +212,11 @@ lemma store_global_success {sig : signature} {i : mcl_address sig} {updates}
     ts
 ).global i = (begin simp [parlang_mcl_global, signature.lean_type_of, lean_type_of], rw a.var_eq, rw h, exact ((map_list updates ts).tlocal.get ⟨var₂, vector_mpr h₂ $ idx.map (eval (map_list updates ts).tlocal)⟩) end) := sorry
 
-def memory_array_update_tid {sig : signature} {n} (var) (s : state n (memory $ parlang_mcl_tlocal sig) (parlang_mcl_global sig)) (expr : expression sig (type_of (sig var))) (m : memory (parlang_mcl_global sig)) := 
+def memory_array_update_tid {sig : signature} {n} (var) (s : state n (memory $ parlang_mcl_tlocal sig) (parlang_mcl_global sig)) (expr : expression sig (type_of (sig.val var))) (m : memory (parlang_mcl_global sig)) := 
 ((list.range_fin n).foldl (λ (m : parlang.memory (parlang_mcl_global sig)) i, m.update ⟨var, eq.mpr sorry v[i]⟩ (eval (s.threads.nth i).tlocal expr))) m
 
 lemma memory_array_update_tid_skip {sig : signature} {n} {var₁ var₂} {s : state n (memory $ parlang_mcl_tlocal sig) (parlang_mcl_global sig)} 
-{expr : expression sig (type_of (sig var₂))} {m : memory (parlang_mcl_global sig)} {i} (a : array_access sig var₁ i) (h : var₁ ≠ var₂) : 
+{expr : expression sig (type_of (sig.val var₂))} {m : memory (parlang_mcl_global sig)} {i} (a : array_access sig var₁ i) (h : var₁ ≠ var₂) : 
 (memory_array_update_tid var₂ s expr m) i = m i := begin
     cases i,
     have : i_fst = var₁ := a.var_eq,
@@ -221,14 +226,13 @@ lemma memory_array_update_tid_skip {sig : signature} {n} {var₁ var₂} {s : st
 end
 
 lemma memory_array_update_tid_success {sig : signature} {n} {var₁ var₂} {s : state n (memory $ parlang_mcl_tlocal sig) (parlang_mcl_global sig)} 
-{expr : expression sig (type_of (sig var₂))} {m : memory (parlang_mcl_global sig)} {i} (a : array_access_tid_to_idx sig var₁ i n) (h : var₁ = var₂) : 
+{expr : expression sig (type_of (sig.val var₂))} {m : memory (parlang_mcl_global sig)} {i} (a : array_access_tid_to_idx sig var₁ i n) (h : var₁ = var₂) : 
 (memory_array_update_tid var₂ s expr m) i = eval (s.threads.nth ⟨_, a.field_per_thread⟩).tlocal (by rw a.to_array_access.var_eq; rw h; exact expr) := begin
     admit,
 end
 
 -- #reduce eval ((map_list [/- λ (s : state sig), state.update' p₁._proof_1 _ (eval s read_tid) s -/] {tlocal := mcl_init 9, global := m''', loads := ∅, stores := ∅}).tlocal) (vector.nth [read_tid] ⟨0, lt_zero_one⟩)
 
-example {sig : signature} {i : mcl_address sig} {s idx} {a} (h : vector ℕ ((sig (i.fst)).type.dim) = vector ℕ ((sig (sigma.fst (⟨s, idx⟩ : mcl_address sig))).type.dim)) : i.snd = eq.mpr h a → i.snd = eq.mpr _ a := sorry
 universe u
 lemma hh {a b : Sort u} (h : a == b) : a = b := begin
     cases h,
@@ -302,7 +306,7 @@ lemma assign_rel : mclp_rel eq p₁ p₂ eq := begin
     split, {
         have : update_global_vars_for_expr read_tid = id := by refl,
         rw this,
-        have : update_global_vars_for_expr (read_tid + (expression.literal_int 1 (show type_of (sig "b") = type_of (sig "b"), by refl))) = id := by refl,
+        have : update_global_vars_for_expr (read_tid + (expression.literal_int 1 (show type_of (sig.val "b") = type_of (sig.val "b"), by refl))) = id := by refl,
         rw this,
         simp,
 
@@ -366,19 +370,7 @@ lemma assign_rel : mclp_rel eq p₁ p₂ eq := begin
                     {
                         apply ha.var_eq,
                     }, {
-                        --apply list_one_eq ha.one_dim,
-                        have : (((sig i.fst).type).dim) = 1 := begin
-                            have : i.fst = "a" := ha.to_array_access.var_eq,
-                            rw this,
-                            rw ← ha.to_array_access.idx_len,
-                            rw ha.one_dim,
-                        end,
-                        --rw this at i_snd,
-                        --dedup,
                         rw vector_map_single,
-                        simp,
-                        unfold array_access_tid_to_idx.tid_to_idx,
-                        simp,
                         cases i,
                         cases ha,
                         cases ha__to_array_access,
@@ -386,26 +378,7 @@ lemma assign_rel : mclp_rel eq p₁ p₂ eq := begin
                         simp at ha__to_array_access_idx_len,
                         dedup,
                         subst ha__to_array_access_var_eq_1,
-                        unfold map_list,
-                        simp,
-                        repeat {rw vector_mpr_singleton},
-                        rw hhh,
-                        rw hhh,
                         apply vector.eq_one,
-                        simp [hhh'],
-                        conv {
-                            congr,
-                            skip,
-                            congr,
-                            congr,
-                            congr,
-                            congr,
-                            congr,
-                            funext,
-                            rw vector_mpr_rfl,
-                        },
-                        rw map,
-                        simp,
                         refl,
                     }
                 }, {
@@ -436,7 +409,8 @@ lemma assign_rel : mclp_rel eq p₁ p₂ eq := begin
                     intros t' ht'n hneqtt',
                     apply store_access_elim_idx, {
                         apply list_neq_elem 0, 
-                        swap, { 
+                        swap, {
+                            rw vector.length_list,
                             rw ha.one_dim,
                             exact lt_zero_one,
                         }, {
